theories/zoo/prelude/tactics.v
@@ -111,10 +111,8 @@ Tactic Notation "solve_proper+" :=
 Tactic Notation "Z_to_nat" ident(x) :=
   let y := fresh x in
   rename x into y;
-  let Heq := fresh in
-  destruct (Z_of_nat_complete y) as (x & Heq); first lia;
-  rewrite -> Heq in *;
-  clear y Heq.
+  destruct (Z_of_nat_complete y) as (x & ->); first lia;
+  try clear y.
 Tactic Notation "Z_to_nat" ident(x) "as" ident(y) :=
   Z_to_nat x;
   rename x into y.
